$$
|tkD - C|^2 = r^2
$$
$$
(tkD - C)(tkD - C) = r^2
$$
$$
(tkd_x - c_x)(tkd_x - c_x) + (tkd_y - c_y)(tkd_y - c_y) = r^2
$$
$$
(t^2k^2d_x^2 -2tkd_xc_x - c_x^2) + (t^2k^2d_y^2 -2tkd_yc_y - c_y^2) = r^2
$$
$$
t^2k^2(d_x^2 + d_y^2) - 2tk(d_xc_x + d_yc_y) - (c_x^2 + c_y^2) = r^2
$$
$$
(d_x^2 + d_y^2)k^2t^2 - 2k(d_xc_x + d_yc_y)t - (c_x^2 + c_y^2 - r^2) = 0
$$
$$
at^2 - bt - c = 0
$$
___
$$
\Delta = b^2 - 4ac
$$
$$
t_1 = \frac {-b - \sqrt{\Delta}}{2a}
$$
$$
t_2 = \frac {-b + \sqrt{\Delta}}{2a}
$$
___
___
$$
(x_1, y_01) - (x_0, y_0)
$$
$$
y = \frac {y_1 - y_0} {x_1 - x_0}x + c
$$
$$
y = mx + c
$$
$$
c = y_0 - mx_0
$$
$$
F(x, y) = mx + c - y
$$

___

|tkD - Cs|^2 = r^2