$$
p_1 + (p_2 - p_1)t
$$
$$
|p_1 + (p_2 - p_1)t|
$$
$$
\sqrt{((p_1.x + (p_2 - p_1).xt)^2 + (p_1.y + (p_2 - p_1).yt)^2)}
$$
$$
(p_1.x + (p_2 - p_1).xt)^2 + (p_1.y + (p_2 - p_1).yt)^2
$$
$$
(p_1.x^2 + 2p_1.x(p_2 - p_1).xt + ((p_2 - p_1).xt)^2) + (p_1.y^2 + 2p_1.y(p_2 - p_1).yt + ((p_2 - p_1).yt)^2)
$$
$$
((p_1.x^2 + p_1.y^2) + (2p_1.x(p_2 - p_1).x + 2p_1.y(p_2 - p_1).y)t + ((p_2.xt - p_1.xt)^2)
$$
$$
((p_1.x^2 + p_1.y^2) + (2p_1.x(p_2 - p_1).x + 2p_1.y(p_2 - p_1).y)t + ((p_2.xt^2 - 2p_2.xp_2.y - p_1.xt^2)
$$
$$
((p_1.x^2 + p_1.y^2) + (2p_1.x(p_2 - p_1).x + 2p_1.y(p_2 - p_1).y)t + (p_2.x + p_2.y- (2p_2.xp_1.x + 2p_2.yp_1.y) - (p_1.x + p_1.y))t^2
$$
$$
(p_2.x + p_2.y- (2p_2.xp_1.x + 2p_2.yp_1.y) - (p_1.x + p_1.y))t^2 + 2p_1.y(p_2 - p_1).y)t + ((p_1.x^2 + p_1.y^2) + (2p_1.x(p_2 - p_1).x
$$


================================

$$
at^2 + bt + c
$$
$$
2at + b = 0
$$
$$
2at = -b
$$
$$
t = -b/2a
$$
